A lot of lemmas for #8 #29 and #30, help wanted at sorry with comment 'HELP', I think it should be true

Automaton.thy
@@ -53,8 +53,8 @@ definition spfStep_h2::" channel set \<Rightarrow> (channel\<rightharpoonup>'m::
 (* spfRestrict wrapper on "h (spfStep_h2 In f)" *)
 (* "h" should be cont, maybe later *)
 (* alternative (\<bottom> \<notin> ran f) *)
-definition spfStep_h1::"channel set \<Rightarrow> channel set \<Rightarrow>((channel\<rightharpoonup>'m::message) \<Rightarrow> 'm SPF) \<Rightarrow>((channel\<rightharpoonup>'m discr\<^sub>\<bottom>)\<rightarrow> 'm SPF)" where
-"spfStep_h1 In Out= (\<lambda> h. (\<Lambda> f. if (In \<subseteq> dom f \<and> (\<forall>c \<in> In. (f \<rightharpoonup> c \<noteq> \<bottom>))) then spfRestrict In Out\<cdot>(h (spfStep_h2 In f)) else spfLeast In Out))"
+definition spfStep_h1::"channel set \<Rightarrow> channel set \<Rightarrow>((channel\<rightharpoonup>'m::message) \<Rightarrow> 'm SPF) \<rightarrow>((channel\<rightharpoonup>'m discr\<^sub>\<bottom>)\<rightarrow> 'm SPF)" where
+"spfStep_h1 In Out= (\<Lambda> h. (\<Lambda> f. if (In \<subseteq> dom f \<and> (\<forall>c \<in> In. (f \<rightharpoonup> c \<noteq> \<bottom>))) then spfRestrict In Out\<cdot>(h (spfStep_h2 In f)) else spfLeast In Out))"
 
 lemma[simp]: "spfDom\<cdot>((\<lambda> f. if (In \<subseteq> dom f \<and> (\<forall>c \<in> In. (f \<rightharpoonup> c \<noteq> \<bottom>))) then spfRestrict In Out\<cdot>(h (spfStep_h2 In f)) else spfLeast In Out)f) = In"
   by simp
@@ -113,6 +113,66 @@ lemma fun_discr_u_spfStep_h2_h: assumes "chain (Y::nat \<Rightarrow>(channel \<r
 
 lemma spfrestrict_below: assumes"x\<sqsubseteq>y" shows "spfRestrict In Out\<cdot>x \<sqsubseteq> spfRestrict In Out\<cdot>y"
   by (simp add: assms monofun_cfun_arg)
+
+lemma obtain_n_for_c:assumes "chain (Y::nat \<Rightarrow> channel\<rightharpoonup>'a discr\<^sub>\<bottom>)" and "((\<Squnion>i. Y i) \<rightharpoonup> c) \<noteq> \<bottom>" obtains n where "(Y n \<rightharpoonup> c) = ((\<Squnion>i. Y i) \<rightharpoonup> c)"
+  by (metis (mono_tags, lifting) assms(1) discr_u_below_eq is_ub_thelub lub_eq_bottom_iff part_the_chain part_the_lub)
+
+lemma exists_n_for_c:assumes "chain (Y::nat \<Rightarrow> channel\<rightharpoonup>'a discr\<^sub>\<bottom>)" and "((\<Squnion>i. Y i) \<rightharpoonup> c) \<noteq> \<bottom>" shows "\<exists>n. (Y n \<rightharpoonup> c) = ((\<Squnion>i. Y i) \<rightharpoonup> c)"
+  by (metis (mono_tags, lifting) assms(1) discr_u_below_eq is_ub_thelub lub_eq_bottom_iff part_the_chain part_the_lub)
+
+lemma discr_u_chain_lubnbot: assumes"chain (Y::nat \<Rightarrow> 'a discr\<^sub>\<bottom>)" and "(\<Squnion>i. Y i) \<noteq>\<bottom>" shows "\<exists>i. Y i \<noteq> \<bottom>"
+  using assms(1) assms(2) lub_eq_bottom_iff by auto
+
+lemma discr_u_chain_lubnbot_forall_c: assumes"chain (Y::nat \<Rightarrow> channel \<Rightarrow> 'a discr\<^sub>\<bottom>)" and "\<forall>c. (\<Squnion>i. Y i) c \<noteq>\<bottom>" shows "\<forall>c. \<exists>i. Y i c \<noteq> \<bottom>" 
+  by (metis (no_types, lifting) assms(1) assms(2) below_refl lub_eq_bottom_iff lub_fun po_class.chain_def)
+    
+lemma discr_u_chain_lubnbot_equiv: assumes"chain (Y::nat \<Rightarrow> channel \<Rightarrow> 'a discr\<^sub>\<bottom>)" shows "((\<Squnion>i. Y i) c \<noteq>\<bottom>) \<longleftrightarrow> (\<exists>i. Y i c \<noteq> \<bottom>)" 
+  by (simp add: assms ch2ch_fun lub_eq_bottom_iff lub_fun) 
+(*
+lemma discr_u_chain_lubnbot_equiv_allc: assumes"chain (Y::nat \<Rightarrow> channel \<Rightarrow> 'a discr\<^sub>\<bottom>)" shows " (\<forall>c. (\<Squnion>i. Y i) c \<noteq>\<bottom>) \<longleftrightarrow> (\<exists>i.\<forall>c. Y i c \<noteq> \<bottom>)"
+  apply(auto)*)
+    
+lemma obtain_n_for_all_c:assumes "chain (Y::nat \<Rightarrow> channel\<rightharpoonup>'a discr\<^sub>\<bottom>)" and "\<forall>c\<in>In. \<exists>i. ((Y i) \<rightharpoonup> c) \<noteq> \<bottom>" and "\<forall>c\<in>In. ((\<Squnion>i. Y i) \<rightharpoonup> c) \<noteq> \<bottom>" shows "\<exists>n. \<forall>c\<in>In. ((Y n)\<rightharpoonup> c) = ((\<Squnion>i. Y i) \<rightharpoonup> c)"
+proof-
+  have chain_Yc:"\<forall>c. chain(\<lambda>i. Y i  \<rightharpoonup> c)"
+    by (metis assms(1) part_the_chain)
+  have "\<forall>c\<in>In. \<exists>i. (Y i  \<rightharpoonup> c) \<noteq> \<bottom>"
+    by (simp add: assms(2))
+  have test1:"\<And>c. c\<in>In \<Longrightarrow> ((\<Squnion>i. Y i) \<rightharpoonup> c) \<noteq> \<bottom>"
+    by(simp add: assms(3))
+  have "\<And>c. c\<in>In  \<Longrightarrow> \<exists>i. (Y i)\<rightharpoonup> c \<noteq> \<bottom>"
+    by (simp add: assms(2))
+  have h1:"\<And>c. c\<in>In \<Longrightarrow>  \<exists>i. (Y i)\<rightharpoonup> c = ((\<Squnion>i. Y i) \<rightharpoonup> c)"
+    using assms(1) assms(3) exists_n_for_c by blast
+  have h2:"\<And>c. c\<in>In \<Longrightarrow> \<exists>i. \<forall>ia\<ge>i. Y ia \<rightharpoonup> c = (Y i)\<rightharpoonup> c"
+  proof -
+    fix c :: channel
+    { fix nn :: "nat \<Rightarrow> nat"
+      have "\<And>f n na c. \<not> chain f \<or> \<not> n \<le> na \<or> (f n\<rightharpoonup>c::channel::'a discr\<^sub>\<bottom>) \<sqsubseteq> f na\<rightharpoonup>c"
+        by (metis part_the_chain po_class.chain_mono)
+      then have "\<exists>n. \<not> n \<le> nn n \<or> Y (nn n)\<rightharpoonup>c = Y n\<rightharpoonup>c"
+        by (metis assms(1) discr_u_below_eq) }
+    then show "\<exists>n. \<forall>na\<ge>n. Y na\<rightharpoonup>c = Y n\<rightharpoonup>c"
+      by meson
+  qed
+  have h3_2:"\<exists>i. \<forall>c\<in>In. Y i \<rightharpoonup> c \<noteq> \<bottom>"(* AHHHHHHHHHHHHHHAHAHAHHHHHHHHHHHHHHHHHH\<And>\<And>\<And>\<And>\<And>\<And>\<And>\<And>\<And>\<And>\<And>\<And>\<And>!11!1\<And>! HELP MEEE*)
+      sorry
+  (*have h3:"\<exists>i. \<forall>c\<in>In. \<forall>ia\<ge>i. Y ia \<rightharpoonup> c = (Y i)\<rightharpoonup> c" 
+    sorry*)
+  then have h4:"\<exists>i. \<forall>c\<in>In. Y i \<rightharpoonup> c = (\<Squnion>i. ((Y i) \<rightharpoonup> c))"
+    using below_lub chain_Yc discr_u_below_eq by blast
+  then have "\<exists>i. \<forall>c\<in>In. (Y i)\<rightharpoonup> c = (\<Squnion>i. Y i)\<rightharpoonup> c"
+    by (metis assms(1) part_the_lub)
+  then show ?thesis
+    by simp
+qed  
+  
+
+
+lemma obtain_n_for_all_ch:assumes "chain (Y::nat \<Rightarrow> channel\<rightharpoonup>'a discr\<^sub>\<bottom>)" and "\<forall>c\<in>In. \<exists>i. ((Y i) \<rightharpoonup> c) \<noteq> \<bottom>" and "\<forall>c\<in>In. ((\<Squnion>i. Y i) \<rightharpoonup> c) \<noteq> \<bottom>" obtains n where "\<forall>c\<in>In. ((Y n)\<rightharpoonup> c) = ((\<Squnion>i. Y i) \<rightharpoonup> c)"
+  using assms(1) assms(2) assms(3) obtain_n_for_all_c by blast
+    
+
     
 (*spfStep_h1 mono cont*)
     
@@ -194,7 +254,7 @@ lemma[simp]:"cont(\<lambda> f. if (In \<subseteq> dom f \<and> (\<forall>c \<in>
         case True
         then have "\<forall>i. In \<subseteq> dom (Y i)" 
           by(simp add:  part_dom_lub a1)
-        have "\<forall>c. chain (\<lambda>i. Y i\<rightharpoonup>c)"
+        have chain_Yc:"\<forall>c. chain (\<lambda>i. Y i\<rightharpoonup>c)"
           using a1 by (metis part_the_chain)
         then have "\<forall>i c. Y i\<rightharpoonup>c \<sqsubseteq> Y (Suc i) \<rightharpoonup>c"
           using po_class.chainE by blast
@@ -202,59 +262,36 @@ lemma[simp]:"cont(\<lambda> f. if (In \<subseteq> dom f \<and> (\<forall>c \<in>
           by (simp add: a1 part_the_lub)
         have "\<exists>c\<in>In. \<forall>i.  Y i\<rightharpoonup>c = \<bottom> \<Longrightarrow>\<exists>c\<in>In.  (\<Squnion>i. Y i) \<rightharpoonup> c = \<bottom>"
           by (simp add: a1 lub_eq_bottom_iff part_the_chain part_the_lub)
-        have "\<forall>c\<in>In. \<exists>i. Y i \<rightharpoonup> c \<noteq> \<bottom>"
+        have h123:"\<forall>c\<in>In. \<exists>i. Y i \<rightharpoonup> c \<noteq> \<bottom>"
           by (metis (mono_tags, lifting) True a1 lub_eq_bottom_iff part_the_chain part_the_lub)
-        then have "\<And>c. c\<in>In \<Longrightarrow>  \<exists>i. Y i \<rightharpoonup> c \<noteq> \<bottom>"
+        then have helper1:"\<And>c. c\<in>In \<Longrightarrow>  \<exists>i. Y i \<rightharpoonup> c \<noteq> \<bottom>"
           by simp
-        have "\<exists>i. \<forall>c\<in>In. Y i \<rightharpoonup> c \<noteq> \<bottom>"
-            sorry          
-         (*proof(cases "\<forall>i. \<exists>c\<in>In. Y i \<rightharpoonup> c = \<bottom>")
-            case True
-            have "\<exists>c\<in>In. (\<Squnion>i. Y i) \<rightharpoonup> c = \<bottom>" 
-            proof(cases "\<forall>c\<in>In. (\<Squnion>i. Y i) \<rightharpoonup> c \<noteq> \<bottom>")
-              case True
-              have "\<forall>c\<in>In. \<exists>i. Y i  \<rightharpoonup> c= (\<Squnion>i. Y i) \<rightharpoonup> c"
-              proof(cases "\<exists>c\<in>In. \<forall>i. Y i \<rightharpoonup> c \<noteq> (\<Squnion>i. Y i)  \<rightharpoonup> c")
-                case True
-                have "\<exists>c\<in>In. \<forall>i. Y i  \<rightharpoonup> c= \<bottom>"
-                  by (metis (mono_tags, lifting) True a1 discr_u_below_eq is_ub_thelub part_the_chain part_the_lub)
-                then show ?thesis
-                  using \<open>\<forall>c\<in>In. \<exists>i. Y i\<rightharpoonup>c \<noteq> \<bottom>\<close> by blast
-              next
-                case False
-                then show ?thesis
-                  by blast
-              qed
-              then show ?thesis 
-                using True 
-                  sorry
-            next
-              case False
-              then show ?thesis 
-                by simp
-            qed
-            then show ?thesis
-              by (smt \<open>\<forall>c\<in>In. \<exists>i. Y i\<rightharpoonup>c \<noteq> \<bottom>\<close> a1 below_fun_def below_option_def discr_u_below_eq is_ub_thelub) 
-          next
-            case False
-            then show ?thesis 
-              by simp
-          qed     *)
-        have "\<And> c. c\<in>In \<Longrightarrow>\<exists>i.  Y i \<rightharpoonup> c = (\<Squnion>i. Y i)\<rightharpoonup>c"
-        proof-
-          fix c::channel
-          assume a11:"c \<in> In"
-          have h1:"\<exists>i.  Y i \<rightharpoonup> c \<noteq> \<bottom>"
-            using \<open>\<exists>i. \<forall>c\<in>In. Y i\<rightharpoonup>c \<noteq> \<bottom>\<close> a11 by auto
-          have h2:"\<forall>c i. Y i\<rightharpoonup>c \<sqsubseteq> (\<Squnion>i. Y i)\<rightharpoonup>c"
-            by (metis  a1 is_ub_thelub part_the_chain part_the_lub)
-          show "\<exists>i.  Y i \<rightharpoonup> c = (\<Squnion>i. Y i)\<rightharpoonup>c" 
-            using discr_u_below_eq h1 h2 by blast
+        have "\<And>x. \<forall>c\<in>In. Y x \<rightharpoonup> c \<noteq> \<bottom> \<Longrightarrow> \<forall>i\<ge>x. \<forall>c\<in>In. Y i \<rightharpoonup> c = Y x \<rightharpoonup> c" 
+          by (metis (mono_tags, lifting) chain_Yc discr_u_below_eq po_class.chain_mono)
+        have helper2:"\<And>x c. Y x \<rightharpoonup> c \<noteq> \<bottom> \<Longrightarrow> \<forall>i\<ge>x. Y i \<rightharpoonup> c = Y x \<rightharpoonup> c" 
+          by (metis (mono_tags, lifting) chain_Yc discr_u_below_eq po_class.chain_mono)
+        then have "\<forall>c. \<exists>i. \<forall>ia\<ge>i. Y ia  \<rightharpoonup> c = Y i  \<rightharpoonup> c"
+          by metis
+        have "\<forall>c\<in>In. \<exists>i. \<forall>ia\<ge>i. Y ia  \<rightharpoonup> c \<noteq> \<bottom>"
+          by (metis helper1 helper2)
+        have "\<forall>c\<in>In. \<exists>i. Y i \<rightharpoonup> c= (\<Squnion>i. Y i) \<rightharpoonup> c"
+        proof -
+          { fix cc :: channel
+            have "\<And>n c. Y n\<rightharpoonup>c \<sqsubseteq> Lub Y\<rightharpoonup>c"
+              by (metis a1 chain_Yc is_ub_thelub part_the_lub)
+            then have "\<exists>n. cc \<notin> In \<or> Y n\<rightharpoonup>cc = Lub Y\<rightharpoonup>cc"
+              by (meson discr_u_below_eq helper1) }
+          then show ?thesis
+            by blast
         qed
-        obtain n where "(In \<subseteq> dom (Y n) \<and> (\<forall>c\<in>In. ((Y n)\<rightharpoonup>c \<noteq> \<bottom>)))"
-          by (meson \<open>\<exists>i. \<forall>c\<in>In. Y i\<rightharpoonup>c \<noteq> \<bottom>\<close> \<open>\<forall>i. In \<subseteq> dom (Y i)\<close>)
-        then have "(\<lambda>i. if (In \<subseteq> dom (Y i) \<and> (\<forall>c\<in>In. ((Y i)\<rightharpoonup>c \<noteq> \<bottom>))) then spfRestrict In Out\<cdot>(h (spfStep_h2 In (Y i))) else spfLeast In Out) n = spfRestrict In Out\<cdot>(h (spfStep_h2 In (Y n)))"
+        then have "\<And> c. c\<in>In \<Longrightarrow>\<exists>i.  Y i \<rightharpoonup> c = (\<Squnion>i. Y i)\<rightharpoonup>c"
           by simp
+        obtain n where "\<forall>c\<in>In. ((Y n)\<rightharpoonup>c = ((\<Squnion>i. Y i) \<rightharpoonup>c))"
+          by(rule obtain_n_for_all_ch[of Y In],simp_all add: a1 True h123)
+        then have "(\<lambda>i. if (In \<subseteq> dom (Y i) \<and> (\<forall>c\<in>In. ((Y i)\<rightharpoonup>c \<noteq> \<bottom>))) then spfRestrict In Out\<cdot>(h (spfStep_h2 In (Y i))) else spfLeast In Out) n = spfRestrict In Out\<cdot>(h (spfStep_h2 In (Y n)))"
+        by (simp add: True \<open>\<forall>i. In \<subseteq> dom (Y i)\<close>)
+        have "In \<subseteq> dom (Y n) \<and> (\<forall>c\<in>In. Y n\<rightharpoonup>c \<noteq> \<bottom>)"
+          by (simp add: True \<open>\<forall>c\<in>In. Y n\<rightharpoonup>c = \<Squnion>i. Y i\<rightharpoonup>c\<close> \<open>\<forall>i. In \<subseteq> dom (Y i)\<close>)
         have "\<forall>i\<ge>n. \<forall>c\<in>In. ((Y i)\<rightharpoonup>c \<noteq> \<bottom>)" 
         proof(auto)
           fix i::nat and c::channel
@@ -314,25 +351,38 @@ lemma[simp]:"cont(\<lambda> f. if (In \<subseteq> dom f \<and> (\<forall>c \<in>
           by(simp add: False False2)
       qed
     qed
+              
+lemma spfStep_h1_mono[simp]:"monofun (\<lambda> h. (\<Lambda> f. if (In \<subseteq> dom f \<and> (\<forall>c \<in> In. (f \<rightharpoonup> c \<noteq> \<bottom>))) then spfRestrict In Out\<cdot>(h (spfStep_h2 In f)) else spfLeast In Out))"
+by(rule monofunI, simp add: below_cfun_def below_fun_def, simp add: spfrestrict_below)
+  
+  
+    
       
-        
-lemma spfStep_h1_mono:"monofun (\<lambda> h. (\<Lambda> f. if (In \<subseteq> dom f \<and> (\<forall>c \<in> In. (f \<rightharpoonup> c \<noteq> \<bottom>))) then spfRestrict In Out\<cdot>(h (spfStep_h2 In f)) else spfLeast In Out))"
-  apply(rule monofunI)
-  sorry
+lemma spfStep_h1_cont[simp]:"cont (\<lambda> h. (\<Lambda> f. if (In \<subseteq> dom f \<and> (\<forall>c \<in> In. (f \<rightharpoonup> c \<noteq> \<bottom>))) then spfRestrict In Out\<cdot>(h (spfStep_h2 In f)) else spfLeast In Out))"
+proof(rule Cont.contI2, simp add: spfStep_h1_mono)  
+  have h0: " \<And>Y x. chain Y \<Longrightarrow> chain (\<lambda>i. Y i (spfStep_h2 In x))"
+    by (simp add: ch2ch_fun)
+  have h1:"\<And>Y x. chain Y \<Longrightarrow>
+           chain (\<lambda>i. \<Lambda> f. if In \<subseteq> dom f \<and> (\<forall>c\<in>In. f\<rightharpoonup>c \<noteq> \<bottom>) then spfRestrict In Out\<cdot>(Y i (spfStep_h2 In f)) else spfLeast In Out) \<Longrightarrow>
+           In \<subseteq> dom x \<Longrightarrow> \<forall>c\<in>In. x\<rightharpoonup>c \<noteq> \<bottom> \<Longrightarrow> spfRestrict In Out\<cdot>((\<Squnion>i. Y i) (spfStep_h2 In x)) \<sqsubseteq> (\<Squnion>i. spfRestrict In Out\<cdot>(Y i (spfStep_h2 In x)))"
+    by(simp add: lub_fun h0 contlub_cfun_arg)
+  show "\<And>Y. chain Y \<Longrightarrow>
+         chain (\<lambda>i. \<Lambda> f. if In \<subseteq> dom f \<and> (\<forall>c\<in>In. f\<rightharpoonup>c \<noteq> \<bottom>) then spfRestrict In Out\<cdot>(Y i (spfStep_h2 In f)) else spfLeast In Out) \<Longrightarrow>
+         (\<Lambda> f. if In \<subseteq> dom f \<and> (\<forall>c\<in>In. f\<rightharpoonup>c \<noteq> \<bottom>) then spfRestrict In Out\<cdot>((\<Squnion>i. Y i) (spfStep_h2 In f)) else spfLeast In Out) \<sqsubseteq>
+         (\<Squnion>i. \<Lambda> f. if In \<subseteq> dom f \<and> (\<forall>c\<in>In. f\<rightharpoonup>c \<noteq> \<bottom>) then spfRestrict In Out\<cdot>(Y i (spfStep_h2 In f)) else spfLeast In Out)"
+    by(simp add: below_cfun_def below_fun_def contlub_cfun_fun, auto, simp add: h1)
+qed
+  
       
-lemma spfStep_h1_cont:"cont (\<lambda> h. (\<Lambda> f. if (In \<subseteq> dom f \<and> (\<forall>c \<in> In. (f \<rightharpoonup> c \<noteq> \<bottom>))) then spfRestrict In Out\<cdot>(h (spfStep_h2 In f)) else spfLeast In Out))"
-  apply(rule Cont.contI2, simp add: spfStep_h1_mono)
-  sorry
       
-      
-lemma[simp]: "spfDom\<cdot>(spfStep_h1 In Out h \<cdot> f) = In"
+lemma[simp]: "spfDom\<cdot>(spfStep_h1 In Out\<cdot> h \<cdot> f) = In"
   by(simp add: spfStep_h1_def)
     
 
-lemma[simp]: "spfRan\<cdot>(spfStep_h1 In Out h \<cdot> f) = Out"
+lemma[simp]: "spfRan\<cdot>(spfStep_h1 In Out\<cdot> h \<cdot> f) = Out"
   by(simp add: spfStep_h1_def)
 
-lemma spfstep_h1_insert: "spfStep_h1 In Out h\<cdot>f = (if (In \<subseteq> dom f \<and> (\<forall>c \<in> In. (f \<rightharpoonup> c \<noteq> \<bottom>))) then spfRestrict In Out\<cdot>(h (spfStep_h2 In f)) else spfLeast In Out)"
+lemma spfstep_h1_insert: "spfStep_h1 In Out\<cdot> h\<cdot>f = (if (In \<subseteq> dom f \<and> (\<forall>c \<in> In. (f \<rightharpoonup> c \<noteq> \<bottom>))) then spfRestrict In Out\<cdot>(h (spfStep_h2 In f)) else spfLeast In Out)"
   by(simp add:  spfStep_h1_def)    
 
 (*spfStep_h1 mono cont end*)     
@@ -340,7 +390,7 @@ lemma spfstep_h1_insert: "spfStep_h1 In Out h\<cdot>f = (if (In \<subseteq> dom 
 thm spfRestrict_def
 (* Skeleton of spfStep. Returns the SPF that switches depending on input *)
 definition spfStep :: "channel set \<Rightarrow> channel set \<Rightarrow> ((channel\<rightharpoonup>'m::message) \<Rightarrow> 'm SPF) \<rightarrow> 'm SPF" where
-"spfStep In Out \<equiv> \<Lambda> h. Abs_SPF (\<Lambda>  sb.  (sbDom\<cdot>sb = In) \<leadsto> (spfStep_h1 In Out h)\<cdot>(sbHdElem\<cdot>sb) \<rightleftharpoons> sb)"
+"spfStep In Out \<equiv> \<Lambda> h. Abs_SPF (\<Lambda>  sb.  (sbDom\<cdot>sb = In) \<leadsto> (spfStep_h1 In Out\<cdot> h)\<cdot>(sbHdElem\<cdot>sb) \<rightleftharpoons> sb)"
 
 
 (* spfStep mono and cont*)
@@ -348,57 +398,184 @@ definition spfStep :: "channel set \<Rightarrow> channel set \<Rightarrow> ((cha
 
 (* spfStep inner SPF spf_well and cont*)
 
-lemma spfStep_inSPF_mono[simp]:"monofun (\<lambda>b. spfStep_h1 In Out h\<cdot>(sbHdElem\<cdot>b) \<rightleftharpoons> b)"
-  apply(rule monofunI) 
-  by (smt below_SPF_def domIff monofun_cfun option.exhaust_sel po_eq_conv sbdom_eq some_below2 spfLeastIDom spf_below_sbdom spf_sbdom2dom)
+lemma spfStep_inSPF_mono[simp]:"monofun (\<lambda>b. spfStep_h1 In Out\<cdot> h\<cdot>(sbHdElem\<cdot>b) \<rightleftharpoons> b)"
+  apply(rule monofunI)
+  by (metis below_SPF_def below_option_def below_refl monofun_cfun monofun_cfun_arg)
 
 
-lemma spfStep_inSPF_cont[simp]:"cont (\<lambda> sb.  (sbDom\<cdot>sb = In) \<leadsto> (spfStep_h1 In Out h)\<cdot>(sbHdElem\<cdot>sb) \<rightleftharpoons> sb)"
+lemma spfStep_inSPF_cont[simp]:"cont (\<lambda> sb.  (sbDom\<cdot>sb = In) \<leadsto> (spfStep_h1 In Out\<cdot> h)\<cdot>(sbHdElem\<cdot>sb) \<rightleftharpoons> sb)"
 proof(rule spf_contI2,rule Cont.contI2,auto)
   fix Y::"nat \<Rightarrow> 'a SB"
   assume chain:"chain Y"
-  assume chain2:"chain (\<lambda>i. spfStep_h1 In Out h\<cdot>(sbHdElem\<cdot>(Y i)) \<rightleftharpoons> Y i)"
-  have h1:"spfStep_h1 In Out h\<cdot>(sbHdElem\<cdot>(\<Squnion>i. Y i)) = (\<Squnion>i. spfStep_h1 In Out h\<cdot>(sbHdElem\<cdot>(Y i)))"
+  assume chain2:"chain (\<lambda>i. spfStep_h1 In Out\<cdot> h\<cdot>(sbHdElem\<cdot>(Y i)) \<rightleftharpoons> Y i)"
+  have h1:"spfStep_h1 In Out\<cdot> h\<cdot>(sbHdElem\<cdot>(\<Squnion>i. Y i)) = (\<Squnion>i. spfStep_h1 In Out\<cdot> h\<cdot>(sbHdElem\<cdot>(Y i)))"
     by(simp add: chain contlub_cfun_fun contlub_cfun_arg)
   have h_true:"sbDom\<cdot>(\<Squnion>i. Y i) = In \<Longrightarrow> \<forall>i. sbDom\<cdot>(Y i) = In"
     by (simp add: chain sbChain_dom_eq2)
   have h_false:"sbDom\<cdot>(\<Squnion>i. Y i) \<noteq> In \<Longrightarrow> \<forall>i. sbDom\<cdot>(Y i) \<noteq> In"
     by (simp add: chain sbChain_dom_eq2)
-  have "(\<Squnion>i. spfStep_h1 In Out h\<cdot>(sbHdElem\<cdot>(Y i))) \<rightleftharpoons> (\<Squnion>i. Y i) = (\<Squnion>i. spfStep_h1 In Out h\<cdot>(sbHdElem\<cdot>(Y i)) \<rightleftharpoons> Y i)"
+  have "(\<Squnion>i. spfStep_h1 In Out\<cdot> h\<cdot>(sbHdElem\<cdot>(Y i))) \<rightleftharpoons> (\<Squnion>i. Y i) = (\<Squnion>i. spfStep_h1 In Out\<cdot> h\<cdot>(sbHdElem\<cdot>(Y i)) \<rightleftharpoons> Y i)" 
     sorry
-  then show "spfStep_h1 In Out h\<cdot>(sbHdElem\<cdot>(\<Squnion>i. Y i)) \<rightleftharpoons> (\<Squnion>i. Y i) \<sqsubseteq> (\<Squnion>i. spfStep_h1 In Out h\<cdot>(sbHdElem\<cdot>(Y i)) \<rightleftharpoons> Y i)"
+  then show "spfStep_h1 In Out\<cdot> h\<cdot>(sbHdElem\<cdot>(\<Squnion>i. Y i)) \<rightleftharpoons> (\<Squnion>i. Y i) \<sqsubseteq> (\<Squnion>i. spfStep_h1 In Out\<cdot> h\<cdot>(sbHdElem\<cdot>(Y i)) \<rightleftharpoons> Y i)"
     by(simp add: h1)
 qed   
     
-lemma spfStep_inSPF_well[simp]:"spf_well (\<Lambda>  sb.  (sbDom\<cdot>sb = In) \<leadsto> (spfStep_h1 In Out h)\<cdot>(sbHdElem\<cdot>sb) \<rightleftharpoons> sb)" 
+lemma spfStep_inSPF_well[simp]:"spf_well (\<Lambda>  sb.  (sbDom\<cdot>sb = In) \<leadsto> (spfStep_h1 In Out\<cdot> h)\<cdot>(sbHdElem\<cdot>sb) \<rightleftharpoons> sb)" 
   proof(rule spf_wellI)
     fix b::"'a SB"
-    assume "b \<in> dom (Rep_cfun (\<Lambda> sb. (sbDom\<cdot>sb = In)\<leadsto>spfStep_h1 In Out h\<cdot>(sbHdElem\<cdot>sb) \<rightleftharpoons> sb))"
-    hence b_def:" b \<in> dom (\<lambda> sb. (sbDom\<cdot>sb = In)\<leadsto>spfStep_h1 In Out h\<cdot>(sbHdElem\<cdot>sb) \<rightleftharpoons> sb)" 
+    assume "b \<in> dom (Rep_cfun (\<Lambda> sb. (sbDom\<cdot>sb = In)\<leadsto>spfStep_h1 In Out\<cdot> h\<cdot>(sbHdElem\<cdot>sb) \<rightleftharpoons> sb))"
+    hence b_def:" b \<in> dom (\<lambda> sb. (sbDom\<cdot>sb = In)\<leadsto>spfStep_h1 In Out\<cdot> h\<cdot>(sbHdElem\<cdot>sb) \<rightleftharpoons> sb)" 
       by simp
     thus "sbDom\<cdot>b = In"
       proof -
         show ?thesis
         by (meson b_def if_then_sbDom)
       qed
-      thus "sbDom\<cdot>(the ((\<Lambda> sb. (sbDom\<cdot>sb = In)\<leadsto>spfStep_h1 In Out h\<cdot>(sbHdElem\<cdot>sb) \<rightleftharpoons> sb)\<cdot>b)) = Out" 
+      thus "sbDom\<cdot>(the ((\<Lambda> sb. (sbDom\<cdot>sb = In)\<leadsto>spfStep_h1 In Out\<cdot> h\<cdot>(sbHdElem\<cdot>sb) \<rightleftharpoons> sb)\<cdot>b)) = Out" 
         by simp
   next
     fix b2::"'a SB"
     assume "sbDom\<cdot>b2 = In"
-    thus "b2 \<in> dom (Rep_cfun (\<Lambda> sb. (sbDom\<cdot>sb = In)\<leadsto>spfStep_h1 In Out h\<cdot>(sbHdElem\<cdot>sb) \<rightleftharpoons> sb))" 
+    thus "b2 \<in> dom (Rep_cfun (\<Lambda> sb. (sbDom\<cdot>sb = In)\<leadsto>spfStep_h1 In Out\<cdot> h\<cdot>(sbHdElem\<cdot>sb) \<rightleftharpoons> sb))" 
       by (simp add: domIff)
 qed
 
 (*spfStep outer cont*)
     
-lemma spfStep_mono:"monofun (\<lambda> h. Abs_SPF (\<Lambda>  sb.  (sbDom\<cdot>sb = In) \<leadsto> (spfStep_h1 In Out h)\<cdot>(sbHdElem\<cdot>sb) \<rightleftharpoons> sb))"
-  sorry
-  
-lemma spfStep_cont:"cont (\<lambda> h. Abs_SPF (\<Lambda>  sb.  (sbDom\<cdot>sb = In) \<leadsto> (spfStep_h1 In Out h)\<cdot>(sbHdElem\<cdot>sb) \<rightleftharpoons> sb))" 
-  sorry
+lemma spfStep_mono[simp]:"monofun (\<lambda> h. Abs_SPF (\<Lambda>  sb.  (sbDom\<cdot>sb = In) \<leadsto> (spfStep_h1 In Out\<cdot> h)\<cdot>(sbHdElem\<cdot>sb) \<rightleftharpoons> sb))"
+proof(rule monofunI, simp add: below_SPF_def below_cfun_def)
+  fix x y::"((channel\<rightharpoonup>'m::message) \<Rightarrow> 'm SPF)"
+  assume a1:"x \<sqsubseteq> y"
+  have h1:"(\<lambda>sb. spfStep_h1 In Out\<cdot>x\<cdot>(sbHdElem\<cdot>sb)) \<sqsubseteq> (\<lambda>sb. spfStep_h1 In Out\<cdot>y\<cdot>(sbHdElem\<cdot>sb))"
+    apply(simp add: below_fun_def)
+    using a1 cfun_below_iff monofun_cfun_arg by blast
+  have h2:"(\<lambda>sb. spfStep_h1 In Out\<cdot>x\<cdot>(sbHdElem\<cdot>sb) \<rightleftharpoons> sb) \<sqsubseteq> (\<lambda>sb. spfStep_h1 In Out\<cdot>y\<cdot>(sbHdElem\<cdot>sb) \<rightleftharpoons> sb)"
+  proof(simp add: below_fun_def,auto)
+    fix xa :: "'m SB"
+    have "\<And>s. spfStep_h1 In Out\<cdot>x\<cdot>(sbHdElem\<cdot>s) \<sqsubseteq> spfStep_h1 In Out\<cdot>y\<cdot>(sbHdElem\<cdot>s)"
+      using fun_below_iff h1 by fastforce
+    then show "spfStep_h1 In Out\<cdot>x\<cdot>(sbHdElem\<cdot>xa) \<rightleftharpoons> xa \<sqsubseteq> spfStep_h1 In Out\<cdot>y\<cdot>(sbHdElem\<cdot>xa) \<rightleftharpoons> xa"
+      by (metis (no_types) below_SPF_def below_option_def below_refl cfun_below_iff)
+  qed
+  show "(\<lambda>sb. (sbDom\<cdot>sb = In)\<leadsto>spfStep_h1 In Out\<cdot>x\<cdot>(sbHdElem\<cdot>sb) \<rightleftharpoons> sb) \<sqsubseteq> (\<lambda>sb. (sbDom\<cdot>sb = In)\<leadsto>spfStep_h1 In Out\<cdot>y\<cdot>(sbHdElem\<cdot>sb) \<rightleftharpoons> sb)"
+    using h2 by (simp add: below_option_def fun_below_iff)
+qed
 
-lemma spfstep_insert: "spfStep In Out\<cdot>h= Abs_SPF (\<Lambda>  sb.  (sbDom\<cdot>sb = In) \<leadsto> (spfStep_h1 In Out h)\<cdot>(sbHdElem\<cdot>sb) \<rightleftharpoons> sb)"
+lemma spf_pref_eq_2: assumes "(f \<sqsubseteq> g)"
+  shows "(f \<rightleftharpoons> a) \<sqsubseteq> (g \<rightleftharpoons> a)" 
+  by (metis assms below_SPF_def below_option_def cfun_below_iff po_eq_conv)
+
+
+lemma getSb_in_h:assumes "chain (Y::nat \<Rightarrow> 'a::message SPF)" shows "(\<Squnion>i. Rep_SPF (Y i))\<cdot> sb = (\<Squnion>i. (Rep_SPF (Y i) \<cdot> sb))"
+  by(subst contlub_cfun_fun, simp_all add: assms)
+    
+    
+lemma getSb_in:assumes "chain Y" shows "(\<Squnion>i. Y i) \<rightleftharpoons> sb = (\<Squnion>i. Y i \<rightleftharpoons> sb)"
+proof(cases "spfDom\<cdot>(\<Squnion>i. Y i) = sbDom\<cdot>sb")
+  case True
+  then have "\<forall>i. spfDom\<cdot>(Y i) = sbDom\<cdot>(sb)"
+    using assms spfdom_eq_lub by auto
+  have chain:"chain (\<lambda>i. Y i \<rightleftharpoons> sb)"
+    by (simp add: op_the_chain assms)
+  have "\<forall>i. Y i  \<rightleftharpoons> sb \<sqsubseteq> (\<Squnion>i. Y i \<rightleftharpoons> sb)"
+    using below_lub chain by blast
+  show ?thesis 
+    (*
+  proof(rule sb_below)
+    show "sbDom\<cdot>((\<Squnion>i. Y i) \<rightleftharpoons> sb) = sbDom\<cdot>(\<Squnion>i. Y i \<rightleftharpoons> sb)"
+      by (metis True \<open>\<forall>i. spfDom\<cdot>(Y i) = sbDom\<cdot>sb\<close> \<open>chain (\<lambda>i. Y i \<rightleftharpoons> sb)\<close> assms sbChain_dom_eq2 spf_ran_2_tsbdom2 spfran_eq_lub)
+  next
+    fix c::channel
+    show "c \<in> sbDom\<cdot>((\<Squnion>i. Y i) \<rightleftharpoons> sb) \<Longrightarrow> ((\<Squnion>i. Y i) \<rightleftharpoons> sb) . c \<sqsubseteq> (\<Squnion>i. Y i \<rightleftharpoons> sb) . c "
+      apply (subst sbgetch_lub, simp_all add: chain)*)
+      sorry
+next
+  case False
+  then have "\<forall>i. spfDom\<cdot>(Y i) \<noteq> sbDom\<cdot>(sb)"
+    using assms spfdom_eq_lub by blast
+  then show ?thesis 
+    by (metis (mono_tags, lifting) spf_pref_eq_2 False assms lub_chain_maxelem option.exhaust_sel po_class.chainE spfdom2sbdom)
+qed
+
+lemma Rep_Abs_CSPF:"cont spf \<and> spf_well (Abs_cfun spf) \<Longrightarrow> Rep_CSPF (Abs_CSPF spf) = spf"
+  by simp   
+    
+  
+lemma spfStep_cont:"cont (\<lambda> h. Abs_SPF (\<Lambda>  sb.  (sbDom\<cdot>sb = In) \<leadsto> (spfStep_h1 In Out\<cdot> h)\<cdot>(sbHdElem\<cdot>sb) \<rightleftharpoons> sb))"
+proof(rule Cont.contI2, simp)
+  fix Y::"nat \<Rightarrow> ((channel\<rightharpoonup>'m::message) \<Rightarrow> 'm SPF)"
+  assume a1: "chain Y"
+  assume a2: "chain (\<lambda>i. Abs_CSPF (\<lambda>sb. (sbDom\<cdot>sb = In)\<leadsto>spfStep_h1 In Out\<cdot>(Y i)\<cdot>(sbHdElem\<cdot>sb) \<rightleftharpoons> sb))"
+  have chain_1:"chain (\<lambda>i. spfStep_h1 In Out\<cdot>(Y i))"
+    using a1 by auto
+  have chain_2:"\<And>x. chain (\<lambda>i. spfStep_h1 In Out\<cdot>(Y i)\<cdot>(sbHdElem\<cdot>x))"
+    using chain_1 by auto
+  have chain_3:"\<And>sb. chain (\<lambda>i. spfStep_h1 In Out\<cdot>(Y i)\<cdot>(sbHdElem\<cdot>sb))"
+    by (simp add: chain_2)
+  have chain_4:"\<And>sb. chain (\<lambda>i. spfStep_h1 In Out\<cdot>(Y i)\<cdot>(sbHdElem\<cdot>sb) \<rightleftharpoons> sb)"
+    by (simp add: chain_2 op_the_chain)
+  have h:"\<forall>sb. spfStep_h1 In Out\<cdot>(\<Squnion>i. Y i)\<cdot>(sbHdElem\<cdot>sb) = (\<Squnion>i. (spfStep_h1 In Out\<cdot>(Y i)\<cdot>(sbHdElem\<cdot>sb)))"
+  by(simp add: a1 chain_1 chain_2 contlub_cfun_arg contlub_cfun_fun contlub_lambda)  
+  have h0_1:"\<forall>sb.  spfStep_h1 In Out\<cdot>(\<Squnion>i. Y i)\<cdot>(sbHdElem\<cdot>sb) \<rightleftharpoons> sb = (\<Squnion>i. (spfStep_h1 In Out\<cdot>(Y i)\<cdot>(sbHdElem\<cdot>sb) \<rightleftharpoons> sb))"
+    apply(subst contlub_cfun_arg, simp add: a1)
+    apply(subst contlub_cfun_fun, simp add: chain_1)
+    by(simp add: getSb_in chain_3)
+  have h0_2:"\<forall>sb. ((sbDom\<cdot>sb = In)\<leadsto>\<Squnion>i. spfStep_h1 In Out\<cdot>(Y i)\<cdot>(sbHdElem\<cdot>sb) \<rightleftharpoons> sb) = (\<Squnion>i. (sbDom\<cdot>sb = In)\<leadsto>spfStep_h1 In Out\<cdot>(Y i)\<cdot>(sbHdElem\<cdot>sb) \<rightleftharpoons> sb)"
+  proof(auto)
+    fix sb::"'m SB"
+    assume a11: "In = sbDom\<cdot>sb"  
+    have h0_21:"((sbDom\<cdot>sb = In)\<leadsto>(\<Squnion>i. spfStep_h1 In Out\<cdot>(Y i)\<cdot>(sbHdElem\<cdot>sb) \<rightleftharpoons> sb)) = (\<Squnion>i. (sbDom\<cdot>sb = In)\<leadsto>spfStep_h1 In Out\<cdot>(Y i)\<cdot>(sbHdElem\<cdot>sb) \<rightleftharpoons> sb)"
+    by(simp add: some_lub_chain_eq chain_4)
+      show"Some (\<Squnion>i. (spfStep_h1 (sbDom\<cdot>sb) Out\<cdot>(Y i)\<cdot>(sbHdElem\<cdot>sb)) \<rightleftharpoons> sb) = (\<Squnion>i. Some ((spfStep_h1 (sbDom\<cdot>sb) Out\<cdot>(Y i)\<cdot>(sbHdElem\<cdot>sb)) \<rightleftharpoons> sb))"
+      using a11 h0_21 by auto
+  qed   (*
+  have cont_lub:"cont (\<lambda>x. \<Squnion>i. (\<Lambda> sb. (sbDom\<cdot>sb = In)\<leadsto>spfStep_h1 In Out\<cdot>(Y i)\<cdot>(sbHdElem\<cdot>sb) \<rightleftharpoons> sb)\<cdot>x)"
+    apply(subst beta_cfun, simp)
+    sorry
+  have spf_well:"spf_well (\<Lambda> x. \<Squnion>i. (\<Lambda> sb. (sbDom\<cdot>sb = In)\<leadsto>spfStep_h1 In Out\<cdot>(Y i)\<cdot>(sbHdElem\<cdot>sb) \<rightleftharpoons> sb)\<cdot>x)"
+    sorry*)
+  have cont_lub:"cont (\<lambda>sb. (sbDom\<cdot>sb = In)\<leadsto>spfStep_h1 In Out\<cdot>(Y i)\<cdot>(sbHdElem\<cdot>sb) \<rightleftharpoons> sb)"
+    by simp
+  have spf_well:"spf_well (\<Lambda> sb. (sbDom\<cdot>sb = In)\<leadsto>spfStep_h1 In Out\<cdot>(Y i)\<cdot>(sbHdElem\<cdot>sb) \<rightleftharpoons> sb)"
+    by simp
+  have chain_h0:"chain (\<lambda>i. \<Lambda> sb. (sbDom\<cdot>sb = In)\<leadsto>spfStep_h1 In Out\<cdot>(Y i)\<cdot>(sbHdElem\<cdot>sb) \<rightleftharpoons> sb)"
+  proof(rule chainI)
+    fix i::nat
+    show "(\<Lambda> sb. (sbDom\<cdot>sb = In)\<leadsto>spfStep_h1 In Out\<cdot>(Y i)\<cdot>(sbHdElem\<cdot>sb) \<rightleftharpoons> sb) \<sqsubseteq> (\<Lambda> sb. (sbDom\<cdot>sb = In)\<leadsto>spfStep_h1 In Out\<cdot>(Y (Suc i))\<cdot>(sbHdElem\<cdot>sb) \<rightleftharpoons> sb)"
+      apply(simp add: below_cfun_def)
+      by (smt below_option_def cfun_below_iff chain_1 fun_belowI po_class.chain_def some_below spf_pref_eq_2)
+  qed    
+  have h0:"Rep_CSPF (\<Squnion>i. Abs_CSPF (\<lambda>sb. (sbDom\<cdot>sb = In)\<leadsto>spfStep_h1 In Out\<cdot>(Y i)\<cdot>(sbHdElem\<cdot>sb) \<rightleftharpoons> sb)) = (\<Squnion>i. (\<lambda>sb. (sbDom\<cdot>sb = In)\<leadsto>spfStep_h1 In Out\<cdot>(Y i)\<cdot>(sbHdElem\<cdot>sb) \<rightleftharpoons> sb))"
+    sorry
+  have h1:"(\<lambda>sb. (sbDom\<cdot>sb = In)\<leadsto>spfStep_h1 In Out\<cdot>(\<Squnion>i. Y i)\<cdot>(sbHdElem\<cdot>sb) \<rightleftharpoons> sb) \<sqsubseteq> Rep_CSPF (\<Squnion>i. Abs_CSPF (\<lambda>sb. (sbDom\<cdot>sb = In)\<leadsto>spfStep_h1 In Out\<cdot>(Y i)\<cdot>(sbHdElem\<cdot>sb) \<rightleftharpoons> sb))"
+    apply(simp add: h0, subst h0_1)
+  proof(rule fun_belowI)
+    fix x::"'m SB"
+    have chain_sb:"chain (\<lambda>i.(\<lambda>sb. (sbDom\<cdot>sb = In)\<leadsto>spfStep_h1 In Out\<cdot>(Y i)\<cdot>(sbHdElem\<cdot>sb) \<rightleftharpoons> sb))"
+    proof(rule chainI)
+      fix i::nat
+      show "(\<lambda>sb. (sbDom\<cdot>sb = In)\<leadsto>spfStep_h1 In Out\<cdot>(Y i)\<cdot>(sbHdElem\<cdot>sb) \<rightleftharpoons> sb) \<sqsubseteq> (\<lambda>sb. (sbDom\<cdot>sb = In)\<leadsto>spfStep_h1 In Out\<cdot>(Y (Suc i))\<cdot>(sbHdElem\<cdot>sb) \<rightleftharpoons> sb)"
+        by (smt below_option_def cfun_below_iff chain_1 fun_belowI po_class.chain_def some_below spf_pref_eq_2)
+    qed 
+    show"(sbDom\<cdot>x = In)\<leadsto>\<Squnion>i. spfStep_h1 In Out\<cdot>(Y i)\<cdot>(sbHdElem\<cdot>x) \<rightleftharpoons> x \<sqsubseteq> (\<Squnion>i. (\<lambda>sb. (sbDom\<cdot>sb = In)\<leadsto>spfStep_h1 In Out\<cdot>(Y i)\<cdot>(sbHdElem\<cdot>sb) \<rightleftharpoons> sb)) x"
+    proof(cases "(sbDom\<cdot>x = In)")
+      case True
+      then show ?thesis
+        by (smt chain_4 chain_sb lub_eq lub_fun po_eq_conv some_lub_chain_eq3)
+    next
+      case False
+      then have "(\<Squnion>i. (\<lambda>sb. (sbDom\<cdot>sb = In)\<leadsto>spfStep_h1 In Out\<cdot>(Y i)\<cdot>(sbHdElem\<cdot>sb) \<rightleftharpoons> sb)) x = None"
+        by (simp add: chain_sb False lub_fun)
+      then show ?thesis
+        by (simp add: False)
+    qed
+  qed
+  show "Abs_CSPF (\<lambda>sb. (sbDom\<cdot>sb = In)\<leadsto>spfStep_h1 In Out\<cdot>(\<Squnion>i. Y i)\<cdot>(sbHdElem\<cdot>sb) \<rightleftharpoons> sb) \<sqsubseteq> (\<Squnion>i. Abs_CSPF (\<lambda>sb. (sbDom\<cdot>sb = In)\<leadsto>spfStep_h1 In Out\<cdot>(Y i)\<cdot>(sbHdElem\<cdot>sb) \<rightleftharpoons> sb))"
+    by(simp add: below_SPF_def below_cfun_def h1)
+qed
+  
+
+lemma spfstep_insert: "spfStep In Out\<cdot>h= Abs_SPF (\<Lambda>  sb.  (sbDom\<cdot>sb = In) \<leadsto> (spfStep_h1 In Out\<cdot> h)\<cdot>(sbHdElem\<cdot>sb) \<rightleftharpoons> sb)"
   by(simp add: spfStep_cont spfStep_def)
 
 thm spfStep_h2_def
